src/lang/Thread.v
@@ -13,7 +13,7 @@ From PromisingLib Require Import Loc.
 
 Require Import Event.
 Require Import Time.
-Require Import Language.
+From PromisingLib Require Import Language.
 
 Require Import View.
 Require Import Cell.
@@ -498,7 +498,7 @@ End Local.
 
 Module Thread.
   Section Thread.
-    Variable (lang:Language.t).
+    Variable (lang:language).
 
     Structure t := mk {
       state: lang.(Language.state);
