src/opt/Adequacy.v
@@ -4,7 +4,7 @@ From Paco Require Import paco.
 
 From PromisingLib Require Import Basic.
 Require Import Event.
-Require Import Language.
+From PromisingLib Require Import Language.
 Require Import View.
 Require Import Cell.
 Require Import Memory.
