src/opt/ReorderStep.v
@@ -9,7 +9,7 @@ From PromisingLib Require Import DenseOrder.
 From PromisingLib Require Import Loc.
 
 Require Import Event.
-Require Import Language.
+From PromisingLib Require Import Language.
 Require Import Time.
 Require Import View.
 Require Import Cell.
