src/opt/SimTrace.v
@@ -8,7 +8,7 @@ From PromisingLib Require Import Axioms.
 From PromisingLib Require Import Basic.
 Require Import Event.
 Require Import Time.
-Require Import Language.
+From PromisingLib Require Import Language.
 Require Import View.
 Require Import Cell.
 Require Import Memory.
